% -*- program: xelatex -*-
\documentclass[10pt]{exam}
\pagestyle{head}
\firstpageheader{\today}{Equation and Inequalities}{Name:\enspace\makebox[1in]{\hrulefill}}
\runningheader{}{}{}
\usepackage{amsmath}
\usepackage{fontspec,realscripts}
\defaultfontfeatures{Ligatures=TeX}
%\setmainfont{Meta Serif Pro}
%\setsansfont{Meta Pro}
\frenchspacing
% - box points & center in the right margin w/ custom setup@point@toks
\boxedpoints
\pointsinrightmargin
\marginbonuspointname{\textsc{up}}
\makeatletter% rewrite setup@point@toks assuming right margins
\def\clap#1{\hbox to 0pt{\hss#1\hss}}% define \clap as per https://www.tug.org/TUGboat/tb22-4/tb72perlS.pdf
\def\setup@point@toks{%
	\point@toks={%
		\rlap{\hskip-\@totalleftmargin
			  \hskip\textwidth
			  \hskip\@rightmargin
			  \hskip-\rightpointsmargin
			  \clap{\padded@point@block}% change \llap to \clap
		}%
		\global \point@toks={}%
	}%
}% end setup@point@toks
\setlength{\rightpointsmargin}{.5in}% assuming the default 1" margins
\makeatother
% - adjust the top and bottom margins
\extraheadheight{.25in}
\extrafootheight{-.5in}
\setlength{\marginparwidth}{1.4in}
% NB: remember to use \newpage after the last question

\usepackage{multicol}

\begin{document}

Solve the following equations or inequalities for \(x\):

\begin{questions}
\begin{multicols}{2}

\question
\( \displaystyle a(2x - 5) + 3 = 4x + 7 \)

\vspace*{1.4in}

\question
\( \displaystyle \frac{bx + 2}{4} = \frac{5x + c}{3} \)

\vspace*{1.4in}

\question
\( \displaystyle 3(a + 2)x - 4 = b(2x + 3) \)

\vspace*{1.4in}

\question
\( \displaystyle \frac{ax + 1}{b} - \frac{3x - 2}{4} = 5 \)

\vspace*{1.4in}

\question
\( \displaystyle 2x - \frac{3}{c} = \frac{ax}{5} + \frac{7}{2} \)

\vspace{1.4in}

\question
\( \displaystyle \frac{3}{a}(2x - 5) > \frac{b}{4}(x + 3) \)

\vspace*{1.4in}

\question
\( \displaystyle \frac{b}{4}(3x - 1) + \frac{5}{c} \leq 2ax - \frac{1}{6} \)

\vspace*{1.4in}

\question
\( \displaystyle a(x - \frac{7}{2}) + \frac{bx}{4} > \frac{5}{6}(2x + 1) \)

\vspace*{1.4in}

\question
\( \displaystyle \frac{cx + 1}{3} - \frac{b}{4} \geq \frac{ax - 2}{6} \)

\vspace*{1.4in}

\question
\( \displaystyle \frac{a}{5}(x - 1) + \frac{2x + b}{3} < \frac{7x - 4}{c} \)

\vspace{1.4in}

\end{multicols}
\end{questions}

\newpage

\begin{multicols*}{2}
\begin{enumerate}
\item \( \displaystyle a(2x - 5) + 3 = 4x + 7 \)

\( \displaystyle 2ax - 5a + 3 = 4x + 7 \)

\( \displaystyle 2ax - 4x = 5a + 4 \)

\( \displaystyle x(2a - 4) = 5a + 4 \)

\( \displaystyle x = \frac{5a + 4}{2a - 4} \)

\item \( \displaystyle \frac{bx + 2}{4} = \frac{5x + c}{3} \)

\( \displaystyle 3(bx + 2) = 4(5x + c) \)

\( \displaystyle 3bx + 6 = 20x + 4c \)

\( \displaystyle 3bx - 20x = 4c - 6 \)

\( \displaystyle x(3b - 20) = 4c - 6 \)

\( \displaystyle x = \frac{4c - 6}{3b - 20} \)

\item \( \displaystyle 3(a + 2)x - 4 = b(2x + 3) \)

\( \displaystyle 3(a + 2)x - 4 = 2bx + 3b \)

\( \displaystyle 3(a + 2)x - 2bx = 3b + 4 \)

\( \displaystyle x(3(a + 2) - 2b) = 3b + 4 \)

\( \displaystyle x = \frac{3b + 4}{3(a + 2) - 2b} \)

\item \( \displaystyle \frac{ax + 1}{b} - \frac{3x - 2}{4} = 5 \)

\( \displaystyle 4(ax + 1) - b(3x - 2) = 20b \)

\( \displaystyle 4ax + 4 - 3bx + 2b = 20b \)

\( \displaystyle (4a - 3b)x = 20b - 4 - 2b \)

\( \displaystyle (4a - 3b)x = 18b - 4 \)

\( \displaystyle x = \frac{18b - 4}{4a - 3b} \)

\item \( \displaystyle 2x - \frac{3}{c} = \frac{ax}{5} + \frac{7}{2} \)

\( \displaystyle 10x - 15 = ax + \frac{35c}{2} \)

\( \displaystyle 10x - ax = \frac{35c}{2} + 15 \)

\( \displaystyle x(10 - a) = \frac{35c}{2} + 15 \)

\( \displaystyle x = \frac{\frac{35c}{2} + 15}{10 - a} \)

\item \( \displaystyle \frac{3}{a}(2x - 5) > \frac{b}{4}(x + 3) \)

\( \displaystyle \frac{6x - 15}{a} > \frac{bx + 3b}{4} \)

\( \displaystyle 24(6x - 15) > a(bx + 3b) \)

\( \displaystyle 144x - 360 > abx + 3ab \)

\( \displaystyle 144x - abx > 360 + 3ab \)

\( \displaystyle x(144 - ab) > 360 + 3ab \)

\( \displaystyle x > \frac{360 + 3ab}{144 - ab} \) (for \( ab \neq 144 \))

\item \( \displaystyle \frac{b}{4}(3x - 1) + \frac{5}{c} \leq 2ax - \frac{1}{6} \)

\( \displaystyle \frac{3bx - b}{4} + \frac{5}{c} \leq 2ax - \frac{1}{6} \)

\( \displaystyle 3bcx - bc + 20 \leq 8acx - 2a \)

\( \displaystyle (3bc - 8ac)x \leq 2a + bc - 20 \)

\( \displaystyle x \leq \frac{2a + bc - 20}{3bc - 8ac} \) (for \( 3bc \neq 8ac \))

\item \( \displaystyle a(x - \frac{7}{2}) + \frac{bx}{4} > \frac{5}{6}(2x + 1) \)

\( \displaystyle ax - \frac{7a}{2} + \frac{bx}{4} > \frac{10x + 5}{6} \)

\( \displaystyle 12ax - 42a + 3bx > 20x + 5 \)

\( \displaystyle (12a + 3b)x > 20x + 42a + 5 \)

\( \displaystyle x(12a + 3b - 20) > 42a + 5 \)

\( \displaystyle x > \frac{42a + 5}{12a + 3b - 20} \) (for \( 12a + 3b \neq 20 \))

\item \( \displaystyle \frac{cx + 1}{3} - \frac{b}{4} \geq \frac{ax - 2}{6} \)

\( \displaystyle 4(cx + 1) - 3b \geq 2(ax - 2) \)

\( \displaystyle 4cx + 4 - 3b \geq 2ax - 4 \)

\( \displaystyle 4cx - 2ax \geq 3b - 8 \)

\( \displaystyle x(4c - 2a) \geq 3b - 8 \)

\( \displaystyle x \geq \frac{3b - 8}{4c - 2a} \) (for \( 4c \neq 2a \))

\item \( \displaystyle \frac{a}{5}(x - 1) + \frac{2x + b}{3} < \frac{7x - 4}{c} \)

\( \displaystyle \frac{a(x - 1)}{5} + \frac{2x + b}{3} < \frac{7x - 4}{c} \)

\( \displaystyle 3a(x - 1) + 5(2x + b) < 15(7x - 4) \)

\( \displaystyle 3ax - 3a + 10x + 5b < 105x - 60 \)

\( \displaystyle 3ax - 95x < -3a + 5b - 60 \)

\( \displaystyle x(3a - 95) < -3a + 5b - 60 \)

\( \displaystyle x < \frac{-3a + 5b - 60}{3a - 95} \) (for \( 3a \neq 95 \))

\end{enumerate}
\end{multicols*}

\end{document}
